wip/confusion around expr.lazy_and and trying to interp
bool expressions directly into Prop instead of requiring
the same rewrites each time

bedrock2/src/bedrock2Examples/LiveVerif/swap.v
@@ -33,6 +33,7 @@ Require Import coqutil.Tactics.autoforward.
 
 (*#[export] not supported in 8.13 yet*)
 Hint Rewrite @word.unsigned_ltu using typeclasses eauto: fwd_rewrites.
+Hint Rewrite @word.signed_lts using typeclasses eauto: fwd_rewrites.
 
 Ltac fwd_rewrites ::= fwd_rewrites_autorewrite.
 
@@ -322,23 +323,6 @@ Section WithParams.
     intros. destruct H. exact H.
   Qed.
 
-  Inductive wp_cmd(call: (string -> trace -> mem -> list word ->
-                          (trace -> mem -> list word -> Prop) -> Prop))
-            (c: cmd)(t: trace)(m: mem)(l: locals)(post: trace -> mem -> locals -> Prop): Prop :=
-    mk_wp_cmd: WeakestPrecondition.cmd call c t m l post -> wp_cmd call c t m l post.
-
-  Lemma weaken_wp_cmd: forall call c t m l (post1 post2: _->_->_->Prop),
-      wp_cmd call c t m l post1 ->
-      (forall t m l, post1 t m l -> post2 t m l) ->
-      wp_cmd call c t m l post2.
-  Proof.
-    intros. constructor. inversion H.
-    eapply WeakestPreconditionProperties.Proper_cmd. 3: eassumption.
-    1: admit.
-    cbv [RelationClasses.Reflexive Morphisms.pointwise_relation Morphisms.respectful Basics.impl].
-    assumption.
-  Admitted. (* TODO some Proper_call and some shelved params *)
-
   Lemma wp_expr_to_dexpr: forall m l e post,
       wp_expr m l e post ->
       exists v, dexpr m l e v /\ post v.
@@ -386,6 +370,215 @@ Section WithParams.
       unfold Morphisms.pointwise_relation, Basics.impl. intros. fwd.
       reflexivity. }
   Qed.
+
+  Definition wp_bool(m: mem)(l: locals)(e: expr)(PTrue PFalse: Prop): Prop :=
+    wp_expr m l e (fun b => (word.unsigned b <> 0 -> PTrue) /\
+                            (word.unsigned b =  0 -> PFalse)).
+
+  Lemma wp_bool_lazy_and: forall m l e1 e2 (PTrue PFalse: Prop),
+      wp_bool m l e1 (wp_bool m l e2 PTrue PFalse) PFalse -> (* PFalse invoked twice!! *)
+      wp_bool m l (expr.lazy_and e1 e2) PTrue PFalse.
+  Proof.
+    unfold wp_bool. intros.
+    eapply wp_lazy_and.
+    eapply weaken_wp_expr. 1: exact H. clear H.
+    cbv beta. intros. fwd. destruct_one_match.
+    - exists (word.of_Z 0).
+      rewrite word.unsigned_of_Z_nowrap by (vm_compute; intuition discriminate). ssplit.
+      + reflexivity.
+      + intuition discriminate.
+      + auto.
+    - specialize (Hp0 E). eapply wp_expr_to_dexpr in Hp0. fwd. unfold dexpr in *.
+      exists v0. ssplit.
+      + constructor. assumption.
+      + assumption.
+      + assumption.
+  Qed.
+
+  Definition interp_bool_binop(bop: bopname)(a b: word): Prop :=
+    match bop with
+    | bopname.lts => word.signed a < word.signed b
+    | bopname.ltu => word.unsigned a < word.unsigned b
+    | bopname.eq => a = b
+    | _ => False
+    end.
+
+  Definition bool_binop_true(bop: bopname)(a b: word): Prop :=
+    match bop with
+    | bopname.lts => word.signed a < word.signed b
+    | bopname.ltu => word.unsigned a < word.unsigned b
+    | bopname.eq => a = b
+    | _ => False
+    end.
+
+  Definition bool_binop_false(bop: bopname)(a b: word): Prop :=
+    match bop with
+    | bopname.lts => word.signed b <= word.signed a
+    | bopname.ltu => word.unsigned b <= word.unsigned a
+    | bopname.eq => a <> b
+    | _ => False
+    end.
+
+  Definition wp_bool_binop(bop: bopname)(a b: word)(PTrue PFalse: Prop): Prop :=
+    match bop with
+    | bopname.lts => (word.signed a < word.signed b -> PTrue) /\
+                     (word.signed b <= word.signed a -> PFalse)
+    | bopname.ltu => (word.unsigned a < word.unsigned b -> PTrue) /\
+                     (word.unsigned b <= word.unsigned a -> PFalse)
+    | bopname.eq => (a = b -> PTrue) /\ (a <> b -> PFalse)
+    | _ => (word.unsigned (interp_binop bop a b) <> 0 -> PTrue) /\
+           (word.unsigned (interp_binop bop a b) =  0 -> PFalse)
+    end.
+
+  (* note: the two props fed to this statement are not inputs (continuations),
+     but outputs, and will be evars *)
+  Inductive interp_bool_bop: bopname -> word -> word -> Prop -> Prop -> Prop :=
+  | interp_bool_lts: forall a b,
+      interp_bool_bop bopname.lts a b
+                      (word.signed a < word.signed b) (word.signed b <= word.signed a)
+  | interp_bool_ltu: forall a b,
+      interp_bool_bop bopname.ltu a b
+                      (word.unsigned a < word.unsigned b) (word.unsigned b <= word.unsigned a)
+  | interp_bool_eq: forall a b,
+      interp_bool_bop bopname.eq a b (a = b) (a <> b).
+
+  (* note: the two props fed to this lemma are not inputs (continuations),
+     but outputs, and will intially be evars, and then be determined by applying
+     a constructor of interp_bool_bop (but v1 and v2 is not in their scope!!) *)
+  Lemma wp_bool_op': forall m l op e1 e2 PTrue PFalse,
+      wp_expr m l e1 (fun v1 =>
+        wp_expr m l e2 (fun v2 =>
+          interp_bool_bop op v1 v2 PTrue PFalse)) ->
+      wp_bool m l (expr.op op e1 e2) PTrue PFalse.
+  Proof.
+    unfold wp_bool. intros. eapply wp_op. eapply weaken_wp_expr. 1: exact H. clear H. cbv beta.
+    intros. eapply weaken_wp_expr. 1: exact H. clear H. cbv beta.
+    intros. inversion H; subst; simpl; split; intros; fwd; auto.
+  Qed.
+
+  Lemma wp_bool_op: forall m l op e1 e2 (PTrue PFalse: Prop),
+      wp_expr m l e1 (fun v1 =>
+        wp_expr m l e2 (fun v2 =>
+          wp_bool_binop op v1 v2 PTrue PFalse)) ->
+      wp_bool m l (expr.op op e1 e2) PTrue PFalse.
+  Proof.
+    unfold wp_bool. intros. eapply wp_op. eapply weaken_wp_expr. 1: exact H. clear H. cbv beta.
+    intros. eapply weaken_wp_expr. 1: exact H. clear H. cbv beta.
+    intros. fwd. unfold interp_binop, wp_bool_binop in *.
+    destruct op; try destruct_one_match.
+    all: rewrite ?word.unsigned_of_Z_nowrap by (vm_compute; intuition discriminate).
+    all: split; intro C; try congruence; fwd; auto.
+  Qed.
+
+  Definition interp_bool_op(bop: bopname)(a b: word): Prop * Prop :=
+    match bop with
+    | bopname.lts => (word.signed a < word.signed b,
+                      word.signed b <= word.signed a)
+    | bopname.ltu => (word.unsigned a < word.unsigned b,
+                      word.unsigned b <= word.unsigned a)
+    | bopname.eq => (a = b, a <> b)
+    | _ => (word.unsigned (interp_binop bop a b) <> 0,
+            word.unsigned (interp_binop bop a b) =  0)
+    end.
+
+  Definition interp_wp_bool_op(bop: bopname)(a b: word)(post: Prop -> Prop -> Prop): Prop :=
+    match bop with
+    | bopname.lts => post (word.signed a < word.signed b)
+                          (word.signed b <= word.signed a)
+    | bopname.ltu => post (word.unsigned a < word.unsigned b)
+                          (word.unsigned b <= word.unsigned a)
+    | bopname.eq => post (a = b) (a <> b)
+    | _ => post (word.unsigned (interp_binop bop a b) <> 0)
+                (word.unsigned (interp_binop bop a b) = 0)
+    end.
+
+  Definition interp_bool_prop(bop: bopname)(a b: word): Prop :=
+    match bop with
+    | bopname.lts => word.signed a < word.signed b
+    | bopname.ltu => word.unsigned a < word.unsigned b
+    | bopname.eq => a = b
+    | _ => word.unsigned (interp_binop bop a b) <> 0
+    end.
+
+  Definition wp_expr_bool(m: mem)(l: locals)(e: expr)(post: Prop -> Prop -> Prop): Prop :=
+    wp_expr m l e (fun b => post (word.unsigned b <> 0) (word.unsigned b = 0)).
+
+  Lemma wp_bool_op'': forall m l op e1 e2 (post: Prop -> Prop -> Prop),
+      wp_expr m l e1 (fun v1 =>
+        wp_expr m l e2 (fun v2 =>
+          interp_wp_bool_op op v1 v2 post)) -> (* v1 and v2 are not in post's scope! *)
+      wp_expr_bool m l (expr.op op e1 e2) post.
+  Proof.
+    unfold wp_expr_bool. intros. eapply wp_op.
+    eapply weaken_wp_expr. 1: exact H. clear H. cbv beta.
+    intros. eapply weaken_wp_expr. 1: exact H. clear H. cbv beta.
+    intros. unfold interp_wp_bool_op, interp_binop in *.
+    destruct op; auto; destruct_one_match; fwd.
+    all: rewrite ?word.unsigned_of_Z_nowrap by (vm_compute; intuition discriminate).
+    all: try (match goal with
+             | HP: ?post ?A ?B |- ?post ?A' ?B' =>
+               replace A' with A; [replace B' with B|]; [exact HP|..]
+         end;
+      apply PropExtensionality.propositional_extensionality; split; intros;
+      (Lia.lia || congruence)).
+  Qed.
+
+  Definition wp_expr_bool_prop(m: mem)(l: locals)(e: expr)(post: Prop -> Prop): Prop :=
+    wp_expr m l e (fun b => post (word.unsigned b <> 0)).
+
+  Lemma wp_bool_op''': forall m l op e1 e2 (post: Prop -> Prop),
+      wp_expr m l e1 (fun v1 =>
+        wp_expr m l e2 (fun v2 =>
+          post (interp_bool_prop op v1 v2))) ->
+      wp_expr_bool_prop m l (expr.op op e1 e2) post.
+  Proof.
+    unfold wp_expr_bool_prop. intros. eapply wp_op.
+    eapply weaken_wp_expr. 1: exact H. clear H. cbv beta.
+    intros. eapply weaken_wp_expr. 1: exact H. clear H. cbv beta.
+    intros. unfold interp_bool_prop, interp_binop in *.
+    destruct op; auto; destruct_one_match; fwd.
+    all: rewrite ?word.unsigned_of_Z_nowrap by (vm_compute; intuition discriminate).
+    all: try (match goal with
+             | HP: ?post ?A |- ?post ?A' =>
+               replace A' with A; [exact HP|..]
+         end;
+      apply PropExtensionality.propositional_extensionality; split; intros;
+      (Lia.lia || congruence)).
+  Qed.
+
+  Lemma wp_bool_lazy_and''': forall m l e1 e2 (post: Prop -> Prop),
+      wp_expr_bool_prop m l e1 (fun B1 => exists B,
+        (B1 -> exists P, wp_expr_bool_prop m l e2 P /\ P B) /\
+        (~B1 -> B) /\
+        (post B)) ->
+      wp_expr_bool_prop m l (expr.lazy_and e1 e2) post.
+  Abort.
+
+  (*
+  Lemma wp_bool_lazy_and''': forall m l e1 e2 (post: Prop -> Prop),
+      wp_expr_bool_prop m l e1 (fun B1 => exists B,
+        (B1 -> wp_expr_bool_prop m l e2 (fun B2 => B2 -> B)) /\
+        (~B1 -> ...) /\
+        (post B) ->
+      wp_expr_bool_prop m l (expr.lazy_and e1 e2) post.
+  *)
+
+  Inductive wp_cmd(call: (string -> trace -> mem -> list word ->
+                          (trace -> mem -> list word -> Prop) -> Prop))
+            (c: cmd)(t: trace)(m: mem)(l: locals)(post: trace -> mem -> locals -> Prop): Prop :=
+    mk_wp_cmd: WeakestPrecondition.cmd call c t m l post -> wp_cmd call c t m l post.
+
+  Lemma weaken_wp_cmd: forall call c t m l (post1 post2: _->_->_->Prop),
+      wp_cmd call c t m l post1 ->
+      (forall t m l, post1 t m l -> post2 t m l) ->
+      wp_cmd call c t m l post2.
+  Proof.
+    intros. constructor. inversion H.
+    eapply WeakestPreconditionProperties.Proper_cmd. 3: eassumption.
+    1: admit.
+    cbv [RelationClasses.Reflexive Morphisms.pointwise_relation Morphisms.respectful Basics.impl].
+    assumption.
+  Admitted. (* TODO some Proper_call and some shelved params *)
 
   Lemma wp_set: forall call x a t m l rest post,
       wp_expr m l a
@@ -475,6 +668,20 @@ Section WithParams.
     intros v (Q1 & Q2 & A & B). eexists. eexists. split. 1: exact A. clear A. cbv beta.
     intros * [? | ?]; fwd; eapply B; eauto.
   Qed.
+
+  Lemma wp_if_bool: forall call c l vars vals thn els rest t m BTrue BFalse Q1 Q2 post,
+      l = reconstruct vars vals ->
+      wp_bool m l c BTrue BFalse ->
+      (BTrue  ->  wp_cmd call thn t m l (fun t' m' l' =>
+                    exists vals', l' = reconstruct vars vals' /\ Q1 t' m' l')) ->
+      (BFalse -> wp_cmd call els t m l (fun t' m' l' =>
+                    exists vals', l' = reconstruct vars vals' /\ Q2 t' m' l')) ->
+      (forall t' m' vals', let l' := reconstruct vars vals' in
+                           BTrue  /\ Q1 t' m' l' \/
+                           BFalse /\ Q2 t' m' l' ->
+                           wp_cmd call rest t' m' l' post) ->
+      wp_cmd call (cmd.seq (cmd.cond c thn els) rest) t m l post.
+  Admitted.
 
   (* The postcondition of the callee's spec will have a concrete shape that differs
      from the postcondition that we pass to `call`, so when using this lemma, we have
@@ -1444,8 +1651,29 @@ Definition sort3: {f: list string * list string * cmd &
 .**/  uintptr_t w0 = load(a);                                                   /**.
 .**/  uintptr_t w1 = load(a+4);                                                 /**.
 .**/  uintptr_t w2 = load(a+8);                                                 /**.
+Ltac cond c ::=
+  lazymatch goal with
+  | cl := current_locals_marker (reconstruct ?vars ?vals) |- wp_cmd ?call _ ?t ?m ?l _ =>
+    (* rapply because eapply inlines `let l'` *)
+    rapply (wp_if_bool call c l vars vals); [cbv [cl current_locals_marker]; reflexivity | ..]
+  end.
+
 .**/  if (w1 < w0 && w1 < w2) {                                                 /**.
+
+{
+  eapply wp_bool_lazy_and.
+  eapply wp_bool_op.
+  eval_expr_step.
+  eval_expr_step.
+  unfold wp_bool_binop. split.
+  (* cps doesn't help because binder that holds result of wp_expr is not in the scope of
+     PTrue/PFalse/merge conditions *)
+
 (*
+Time rewrite @word.unsigned_ltu by typeclasses eauto.
+(* hopefully faster in 8.15 thanks to https://github.com/coq/coq/pull/14253 *)
+
+fwd_step.
 .**/    store(a, w1);                                                           /**.
 .**/    w1 = w0;                                                                /**.
 .**/  } else if (w2 < w0 && w2 < w1) {                                          /**.
